Removed sflib dependency

cem_cbn_bisim.v
@@ -1,10 +1,21 @@
-Require Import bisim.
+Require Import bisim db List.
 Require cem cbn.
 
 Inductive state_rel : relation cem.configuration cbn.configuration := 
-  | empty : 
+  | init : forall t e,
+           deBruijn t e -> 
+           state_rel (cem.st nil (cem.close e 0)) (cbn.st nil t)
+  | step : forall a b a' b',
+           state_rel a b ->
+           cem.step a a' -> 
+           cbn.step b b' ->
+           state_rel a' b'.
 
-Theorem cem_cbn_bisim : bisim
-  v b
-
-
+Theorem cem_cbn_bisim : bisim state_rel cem.step cbn.step.
+unfold bisim.
+intros. split. 
+  intros. induction H0. apply IHstep in H. induction H. induction H. inversion H0. subst. 
+assert app_cons_not_nil. rewrite <-
+app_cons_not_nil in H. 
+destruct H0. inversion H. rewrite app_cons_not_nil in H.
+assert False. destruct H0. 
